Prove tuple weak congruence

src/Core_Erlang_Weak_Equivalence.v
@@ -646,6 +646,204 @@ End equivalence_relation.
 
 Section congruence.
 
+Lemma nth_last_eq {A : Type} (l : list A) : forall e,
+  forall d1 d2, nth (length l) (e::l) d1 = last (e::l) d2.
+Proof.
+  induction l using list_length_ind; intros.
+  destruct l.
+  * simpl. auto.
+  * simpl. destruct (length l) eqn:HH.
+    - apply length_zero_iff_nil in HH. subst. auto.
+    - pose (element_exist _ _ (eq_sym HH)). destruct e0. destruct H0. subst.
+      inversion HH. apply H. simpl. lia.
+Qed.
+
+Definition transform_with {A : Type} (l : list (list A)) (addition : list A) : list (list A) :=
+  map (fun x => addition ++ x) l.
+
+
+Lemma effect_extension_exprlist_fbs exps :
+forall c env id0 eff0 id' res eff',
+  fbs_values (fbs_expr c) env id0 exps eff0 = Result id' res eff'
+->
+  exists l, eff' = eff0 ++ l.
+Proof.
+  induction exps; intros.
+  * exists []. simpl in H. inversion H. subst. rewrite app_nil_r. auto.
+  * simpl in H. destruct (fbs_expr c env id0 a eff0) eqn:D1. destruct res0.
+    destruct v. congruence. destruct v0. 2: congruence. 3-4: congruence.
+    - apply fbs_expr_correctness in D1 as D1'.
+      apply effect_extension_expr in D1'. destruct D1'. subst.
+      destruct (fbs_values (fbs_expr c) env id exps (eff0 ++ x)) eqn:D2.
+      destruct res0. 3-4: congruence.
+      + inversion H. subst. apply IHexps in D2. destruct D2. subst.
+        exists (x ++ x0). rewrite <- app_assoc. auto.
+      + inversion H. subst. apply IHexps in D2. destruct D2. subst.
+        exists (x ++ x0). rewrite <- app_assoc. auto.
+    - inversion H. subst.
+      apply fbs_expr_correctness in D1 as D1'.
+      apply effect_extension_expr in D1'. destruct D1'. subst.
+      exists x. auto.
+Qed.
+
+Lemma effectlist_irrelevant_exprlist_fbs exps :
+forall c env id0 id' res eff0 ad,
+  fbs_values (fbs_expr c) env id0 exps eff0 = Result id' res (eff0 ++ ad)
+->
+  forall eff1, 
+  fbs_values (fbs_expr c) env id0 exps eff1 = Result id' res (eff1 ++ ad).
+Proof.
+  intros. apply expr_list_effectlist_irrelevant with eff0. 2: auto.
+  intros. eapply effectlist_irrelevant_fbs_expr. exact H0.
+Qed.
+
+Lemma exprlist_cong_fbs (l : list Expression) :
+forall (l' : list Expression) clock env id eff id' res eff',
+   length l = length l' ->
+   (forall i, i < length l -> weakly_equivalent (nth i l ErrorExp) (nth i l' ErrorExp)) ->
+  fbs_values (fbs_expr clock) env id l eff = Result id' res eff'
+->
+  exists cl eff'', fbs_values (fbs_expr cl) env id l' eff = Result id' res eff'' /\ Permutation eff' eff''.
+Proof.
+  induction l; intros.
+  * inversion H1. subst. exists clock, eff'.
+    apply eq_sym, length_zero_iff_nil in H. subst. simpl. split; auto.
+  * pose (element_exist _ _ H). destruct e. destruct H2. subst.
+    pose (EQ0 := H0 0 (Nat.lt_0_succ _)). simpl in EQ0.
+    simpl in H1. destruct (fbs_expr clock env id a eff) eqn:D1.
+    destruct res0. destruct v. congruence. destruct v0. 2: congruence.
+    3-4: congruence.
+    - destruct (fbs_values (fbs_expr clock) env id0 l eff0) eqn:D2.
+      destruct res0. 3-4: congruence.
+      + apply fbs_expr_correctness in D1.
+        apply effect_extension_expr in D1 as HH. destruct HH. subst.
+        apply EQ0 in D1. destruct D1, H2.
+        apply effect_extension_expr in H2 as HH.
+        apply fbs_soundness in H2.
+        destruct H2, HH. subst.
+
+        apply effect_extension_exprlist_fbs in D2 as D2'. destruct D2'. subst.
+        apply IHl with (l' := x0) in D2. destruct D2, H4, H4.
+        2: simpl in H; lia.
+        2: { intros. epose (H0 (S i) _). exact w. Unshelve. simpl. lia. }
+        apply effect_extension_exprlist_fbs in H4 as HH. destruct HH. subst.
+        inversion H1. subst.
+
+        exists (x3 + x5), (eff ++ x4 ++ x7). simpl.
+        apply bigger_clock_expr with (clock' := x3 + x5) in H2. 2: lia.
+        rewrite H2.
+        apply bigger_clock_list with (clock' := x3 + x5) in H4. 2: lia.
+        apply effectlist_irrelevant_exprlist_fbs with (eff1 := eff ++ x4) in H4.
+        2: { intros. apply clock_increase_expr. exact H6. }
+        rewrite H4. split; rewrite <- app_assoc.
+        ** auto.
+        ** apply Permutation_app_head. apply Permutation_app_inv_l in H3.
+           apply Permutation_app_inv_l in H5. apply Permutation_app; auto.
+      + apply fbs_expr_correctness in D1.
+        apply effect_extension_expr in D1 as HH. destruct HH. subst.
+        apply EQ0 in D1. destruct D1, H2.
+        apply effect_extension_expr in H2 as HH.
+        apply fbs_soundness in H2.
+        destruct H2, HH. subst.
+
+        apply effect_extension_exprlist_fbs in D2 as D2'. destruct D2'. subst.
+        apply IHl with (l' := x0) in D2. destruct D2, H4, H4.
+        2: simpl in H; lia.
+        2: { intros. epose (H0 (S i) _). exact w. Unshelve. simpl. lia. }
+        apply effect_extension_exprlist_fbs in H4 as HH. destruct HH. subst.
+        inversion H1. subst.
+
+        exists (x3 + x5), (eff ++ x4 ++ x7). simpl.
+        apply bigger_clock_expr with (clock' := x3 + x5) in H2. 2: lia.
+        rewrite H2.
+        apply bigger_clock_list with (clock' := x3 + x5) in H4. 2: lia.
+        apply effectlist_irrelevant_exprlist_fbs with (eff1 := eff ++ x4) in H4.
+        2: { intros. apply clock_increase_expr. exact H6. }
+        rewrite H4. split; rewrite <- app_assoc.
+        ** auto.
+        ** apply Permutation_app_head. apply Permutation_app_inv_l in H3.
+           apply Permutation_app_inv_l in H5. apply Permutation_app; auto.
+    - inversion H1. subst. apply fbs_expr_correctness in D1.
+      apply EQ0 in D1. destruct D1. destruct H2.
+      apply fbs_soundness in H2. destruct H2. exists x2, x1.
+      simpl. rewrite H2; auto.
+Qed.
+
+(* Lemma exprlist_congruence (l : list Expression) :
+forall (l' : list Expression) vals eff0 ids env id eff,
+  (forall i, i < length l -> weakly_equivalent (nth i l ErrorExp) (nth i l' ErrorExp))
+  ->
+  (forall i : nat,
+       i < length l ->
+       | env, nth_def ids id 0 i, nth i l ErrorExp, eff ++ nth_def eff0 [] [] i | -e>
+       | nth_def ids id 0 (S i), inl [nth i vals ErrorValue], eff ++ nth_def eff0 [] [] (S i) |)
+  ->
+  length l = length l' ->
+  length l = length vals ->
+  length l = length eff0 ->
+  length l = length ids
+->
+  (exists effs, length l = length effs /\ 
+    (forall i : nat, i < length l' ->
+    | env, nth_def ids id 0 i, nth i l' ErrorExp, eff ++ nth_def effs [] [] i | -e>
+    | nth_def ids id 0 (S i), inl [nth i vals ErrorValue], eff ++ nth_def effs [] [] (S i)| /\
+    Permutation (nth i eff0 []) (nth i effs []))
+  ).
+Proof.
+  induction l; intros.
+  * simpl length in *. repeat unfold_list_once. exists []. split. 2: split.
+    all: auto;
+    inversion H1.
+  * pose (element_exist _ _ H1). pose (element_exist _ _ H2).
+    pose (element_exist _ _ H3). pose (element_exist _ _ H4).
+    destruct e as [e']. destruct e0 as [v']. destruct e1 as [eff1].
+    destruct e2 as [id1]. destruct H5, H6, H7, H8. subst.
+    pose (E := H0 0 (Nat.lt_0_succ (length l))). simpl in E.
+    apply effect_extension_expr in E as E'. destruct E'. subst.
+    inversion H1. inversion H2. inversion H3. inversion H4.
+    pose (W := H 0 (Nat.lt_0_succ _)). simpl in W. apply W in E. clear W. destruct E, H6.
+    apply effect_extension_expr in H6 as HH'. destruct HH'. subst.
+    epose (IHl x x0 (transform_with x1 x3) x2 env id1 (eff ++ x5) _ _ H7 H8 _ H10). destruct e, H12.
+    eexists (x5 :: x4). split. 2: split.
+    - simpl. (* unfold transform_with. rewrite map_length. *) lia.
+    - intros. destruct i.
+      + simpl. rewrite app_nil_r. rewrite app_nil_r in H6. exact H6.
+      + simpl in H14. apply Lt.lt_S_n in H14. epose (P := H13 i H14).
+        simpl in P. unfold transform_with. simpl.
+        destruct i.
+        ** simpl in P. admit.
+        
+        (* epose (P1 := @nth_error_nth' _ x4 0 [] _).
+           apply map_nth_error with (f := fun x => x5 ++ x) in P1.
+           pose (P2 := @nth_error_nth _ _ _ _ [] P1).
+           rewrite P2. simpl in P. rewrite app_nil_r in P.
+           rewrite <- app_assoc in P. apply P. *)
+        ** epose (P1 := @nth_error_nth' _ x4 (S i) [] _).
+           apply map_nth_error with (f := fun x => x5 ++ x) in P1.
+           pose (P2 := @nth_error_nth _ _ _ _ [] P1).
+           rewrite P2. simpl in P.
+           epose (P1' := @nth_error_nth' _ x4 i [] _).
+           apply map_nth_error with (f := fun x => x5 ++ x) in P1'.
+           pose (P2' := @nth_error_nth _ _ _ _ [] P1').
+           rewrite P2'.
+           rewrite <- app_assoc, <- app_assoc in P. apply P.
+    - destruct i.
+      + simpl. rewrite app_nil_r in H11. apply Permutation_app_inv_l in H11.
+        auto.
+      + simpl in H14. apply Lt.lt_S_n in H14. pose (P := H13 i H14).
+        destruct P. simpl.
+        epose (P1' := @nth_error_nth' _ x4 i [] _).
+        apply map_nth_error with (f := fun x => x5 ++ x) in P1'.
+        pose (P2' := @nth_error_nth _ _ _ _ [] P1').
+        unfold transform_with. rewrite P2'. rewrite app_assoc. auto.
+Unshelve.
+ ** intros. epose (H (S i) _). exact w. Unshelve. simpl. lia.
+ ** intros. epose (H0 (S i) (Lt.lt_n_S _ _ H11)). simpl in e.
+    destruct i.
+    -- simpl.
+ ** simpl. simpl in e.
+Admitted. *)
+
 Theorem ECons_weak_congr hd tl : forall hd' tl',
   weakly_equivalent hd hd' -> weakly_equivalent tl tl'
 ->
@@ -698,6 +896,7 @@ Proof.
   * eapply A. exact (weak_sym H). exact (weak_sym H0). exact H1.
 Qed.
 
+
 Theorem ETuple_weak_congr (l : list Expression) : forall (l' : list Expression),
   length l = length l' ->
   (forall i, i < length l -> weakly_equivalent (nth i l ErrorExp) (nth i l' ErrorExp))
@@ -708,30 +907,34 @@ Proof.
     length l = length l' ->
     (forall i, i < length l -> weakly_equivalent (nth i l ErrorExp) (nth i l' ErrorExp))
     ->
-    |env, id, ETuple l, eff| -s> |id', res, eff'|
+    (exists clock, fbs_single clock env id (ETuple l) eff = Result id' res eff')
     ->
-    |env, id, ETuple l', eff| -s> |id', res, eff'|). {
-  intros. unfold weakly_equivalent, weakly_equivalent_single in *.
-  * inversion H1; subst; rewrite H in *.
-    - eapply eval_tuple.
-      + exact H3.
-      + exact H4.
-      + exact H5.
-      + intros. pose (H6 i H2). apply H0 in e. 2: auto. auto.
-      + auto.
-      + auto.
-    - eapply eval_tuple_ex.
-      + exact H3.
-      + reflexivity.
-      + exact H5.
-      + exact H6.
-      + intros. pose (H7 j H2). apply H0 in e. 2: lia. auto.
-      + apply H0 in H10. auto. lia.
+    exists clock eff'', fbs_single clock env id (ETuple l') eff = Result id' res eff'' /\ Permutation eff' eff''). {
+  intros. destruct H1, x.
+  inversion H1.
+  simpl in H1. destruct (fbs_values (fbs_expr x) env id l0 eff) eqn: D1.
+  destruct res0. 3-4: congruence.
+  * inversion H1.
+    apply exprlist_cong_fbs with (l' := l') in D1. destruct D1, H2, H2.
+    subst.
+    exists (S x0), x1. split; auto.
+    2-3: auto.
+    simpl. rewrite H2. reflexivity.
+  * inversion H1.
+    apply exprlist_cong_fbs with (l' := l') in D1. destruct D1, H2, H2.
+    subst.
+    exists (S x0), x1. split; auto.
+    2-3: auto.
+    simpl. rewrite H2. reflexivity.
   }
   split; intros.
-  * eapply A. exact H. auto. auto.
-  * eapply A. symmetry. exact H. intros. rewrite <- H in *.
-    apply weak_sym. auto. auto.
+  * apply fbs_soundness in H1. eapply A in H; auto. 2: exact H1. 
+    destruct H, H, H.
+    exists x0. apply fbs_single_correctness in H. split. exact H. auto.
+  * apply fbs_soundness in H1. eapply A with (l' := l) in H1; auto.
+    2: { intros. apply weak_sym. apply H0. lia. }
+    destruct H1, H1, H1.
+    exists x0. apply fbs_single_correctness in H1. split. exact H1. auto.
 Qed.
 
 Theorem ECall_weak_congr (f : string) (l : list Expression) : forall (l' : list Expression),
@@ -1010,14 +1213,37 @@ Theorem ELet_weak_congr (e1 e2 : Expression) vl : forall (e1' e2' : Expression),
 ->
   weakly_equivalent_single (ELet vl e1 e2) (ELet vl e1' e2').
 Proof.
-  intros. unfold weakly_equivalent, weakly_equivalent_single in *.
+  assert (A : forall env id e1 e1' e2 e2' vl eff id' res eff',
+    weakly_equivalent e1 e1' -> weakly_equivalent e2 e2' ->
+    | env, id, ELet vl e1 e2, eff | -s> | id', res, eff' |
+  ->
+    exists eff'', | env, id, ELet vl e1' e2', eff | -s> |id', res, eff'' | /\ Permutation eff' eff''
+  ).
+  {
+    intros. unfold weakly_equivalent in *. destruct H, H0.
+    inversion H1; subst.
+    * apply effect_extension_expr in H9 as H9'. destruct H9'. subst.
+      apply effect_extension_expr in H15 as H15'. destruct H15'. subst.
+      apply H in H9. destruct H9, H4.
+      apply effect_extension_expr in H4 as H4'. destruct H4'. subst.
+      apply effectlist_irrelevant_expr with (eff0 := eff ++ x2) in H15.
+      apply H0 in H15. destruct H15, H6.
+      apply effect_extension_expr in H6 as H6'. destruct H6'. subst.
+      exists ((eff ++ x2) ++ x3). split. eapply eval_let.
+      - exact H4.
+      - assumption.
+      - exact H6.
+      - apply Permutation_app.
+        + apply Permutation_app_head. apply Permutation_app_inv_l in H5. assumption.
+        + apply Permutation_app_inv_l in H7. assumption.
+    * apply effect_extension_expr in H13 as H13'. destruct H13'. subst.
+      apply H in H13. destruct H13, H4.
+      apply effect_extension_expr in H4 as H4'. destruct H4'. subst.
+      exists (eff ++ x1). split; [ eapply eval_let_ex; auto | auto ].
+  }
   split; intros.
-  * inversion H1; subst.
-    - eapply eval_let. apply H. exact H7. auto. apply H0. exact H13.
-    - eapply eval_let_ex. apply H. auto.
-  * inversion H1; subst.
-    - eapply eval_let. apply H. exact H7. auto. apply H0. exact H13.
-    - eapply eval_let_ex. apply H. auto.
+  * eapply A. exact H. exact H0. exact H1.
+  * eapply A. exact (weak_sym H). exact (weak_sym H0). exact H1.
 Qed.
 
 Theorem ESeq_weak_congr e1 e2 e1' e2' :
@@ -1060,8 +1286,10 @@ Theorem ELetRec_weak_congr (exp : Expression) l : forall (exp' : Expression),
 Proof.
   intros. unfold weakly_equivalent, weakly_equivalent_single in *.
   split; intros.
-  * inversion H0. subst. eapply eval_letrec. apply H. exact H9.
-  * inversion H0. subst. eapply eval_letrec. apply H. exact H9.
+  * inversion H0. subst. destruct H. apply H in H9. destruct H9, H2.
+    exists x. split; auto. eapply eval_letrec; auto.
+  * inversion H0. subst. destruct H. apply H1 in H9. destruct H9, H2.
+    exists x. split; auto. eapply eval_letrec; auto.
 Qed.
 
 Theorem EMap_weak_congr (l : list (Expression * Expression)) : 
@@ -1130,12 +1358,37 @@ Proof.
     weakly_equivalent e3 e3' ->
     |env, id, ETry e1 vl1 e2 vl2 e3, eff | -s> |id', res, eff'|
     ->
-    |env, id, ETry e1' vl1 e2' vl2 e3', eff| -s> |id', res, eff'|
+    (exists eff'', |env, id, ETry e1' vl1 e2' vl2 e3', eff| -s> |id', res, eff''| /\ Permutation eff' eff'')
   ).
   {
-    intros. inversion H2; subst.
-    * eapply eval_try. apply H. exact H14. auto. apply H0. exact H16.
-    * eapply eval_catch. apply H. exact H14. apply H1. exact H15.
+    intros. unfold weakly_equivalent in *. destruct H, H0, H1. inversion H2; subst.
+    * apply effect_extension_expr in H17 as H17'. destruct H17'. subst.
+      apply effect_extension_expr in H19 as H19'. destruct H19'. subst.
+      apply H in H17. destruct H17, H6.
+      apply effect_extension_expr in H6 as H6'. destruct H6'. subst.
+      apply H0 in H19. destruct H19, H8.
+      apply effect_extension_expr in H8 as H8'. destruct H8'. subst.
+      apply effectlist_irrelevant_expr with (eff0 := eff ++ x2) in H8.
+      exists (eff ++ x2 ++ x3). split. eapply eval_try.
+      - exact H6.
+      - auto.
+      - rewrite app_assoc. exact H8.
+      - rewrite <- app_assoc. apply Permutation_app_head. apply Permutation_app.
+        + apply Permutation_app_inv_l in H7. auto.
+        + apply Permutation_app_inv_l in H9. auto.
+    * apply effect_extension_expr in H17 as H17'. destruct H17'. subst.
+      apply effect_extension_expr in H18 as H18'. destruct H18'. subst.
+      apply H in H17. destruct H17, H6.
+      apply effect_extension_expr in H6 as H6'. destruct H6'. subst.
+      apply H1 in H18. destruct H18, H8.
+      apply effect_extension_expr in H8 as H8'. destruct H8'. subst.
+      apply effectlist_irrelevant_expr with (eff0 := eff ++ x2) in H8.
+      exists (eff ++ x2 ++ x3). split. eapply eval_catch.
+      - exact H6.
+      - rewrite app_assoc. exact H8.
+      - rewrite <- app_assoc. apply Permutation_app_head. apply Permutation_app.
+        + apply Permutation_app_inv_l in H7. auto.
+        + apply Permutation_app_inv_l in H9. auto.
   }
   split; intros.
   * eapply A. exact H. exact H0. exact H1. auto.
